Valaig.lean
@@ -1,3 +1,5 @@
+module
+
 import Valaig.Aig
-import Valaig.Aiger
-import Valaig.External
+import Valaig.ForLean
+import Valaig.Data
